---
title: EC2104 Tutorial 3 solution
author: ling
output:
    beamer_presentation:
        slide_level: 2
        toc: false
theme: "Madrid"
---

# Question 3(a)

Given: $\dot{S}=-aS(t)$,
WTS: $S(t) = S_0e^{at}$

1. We know $\dot{S} = \frac{dS}{dt}$, rearranging the given
   term we have $\frac{\left( \frac{dS}{dt} \right)}{S}=-a$
2. Now, consider $f(S)=\ln(S)$, we have $\frac{df}{dt} = \frac{1}{S}\cdot \frac{dS}{dt}$ by chain rule
3. Observe results from (1) and (2). We note that
   $$
   \frac{d\ln(S)}{dt} = \frac{\left(\frac{dS}{dt}\right)}{S} = \frac{\dot{S}}{S} = -a
   $$
4. Now, solve for the differential (integrate both side wrt t)
   \begin{align*}
   \Rightarrow \ln(S) &= -at + C\\
   \Rightarrow S(t) &= e^{-at+C} = e^C\cdot e^{-at}
   \end{align*}
5. When $t=0, S(0)=S_0 \Rightarrow e^C \cdot e^{0} = S_0
   \Rightarrow e^C = S_0$
6. Therefore
   $$
   \Rightarrow S(t) = S_0 e^{-at} \text{ (shown)}
   $$


# Question 4(a)

Amount $A(0)$ is invested with $p$% yearly interest, ask
$A(t) :=$ value of investment after $t$ years

1. We know the rate of change over time (from the question)
   $$
   \frac{dA(t)}{dt} = p\cdot A(t)
   $$
2. Expressing the equation as differential equation and
   integrate both side
   $$
   \frac{1}{A(t)}dA(t) = p dt \Rightarrow \int\frac{1}{A(t)}dA(t) = \int p dt
   $$
3. Solution:
   - $\Rightarrow \ln(A(t)) = pt + C$
   - $A(t) = e^{pt+C} = e^C\cdot e^{pt}$
   - Since $A(0) = e^C\Rightarrow A(t) = A(0)e^{pt}$
