---
title: EC2104 Lecture 4 - Integration
author: ling
output:
    beamer_presentation:
        slide_level: 3
        toc: false
theme: "Madrid"
---

# Integration

\begin{block}{Indefinite integrals}
If $F'(x) = f(x)$, then $\int f(x) dx = F(x) + C$.
Given $A = F(0) + C \Rightarrow C = A - F(0)$
\end{block}

\begin{block}{Definite integrals}
When $F'(x)=f(x)$ for all $x\in(a, b)$, the definite integral
of $f$ over $[a, b]$ is $\int_a^b f(x) dx = F(b) - F(a)$
\end{block}

\begin{block}{Integration as Area Under Curve}
Let $A(t)$ be a function measures the area under the graph
of $f$ over the interval
$[a, t] \Rightarrow A(t)=\int_a^b f(t)dt$
\end{block}

## Integration as Area Under Curve

Consider:
Find area under the curve for $f(x)=cos(x)$ for $x\in[0, \pi]$

Note:

- $\int cos(x) dx = sin(x) + C$
- When finding area under a curve, one need to 
  know which area are under the $x-axis$
- For area under the $x-axis$, take $-\int f(x) dx$
  instead

Wrong method:
$$
\int_0^\pi cos(x) dx = sin(\pi) - sin(0) = 0
$$

Correct method:
$$
\int_0^{\pi/2} cos(x) dx
- \int_{\pi/2}^\pi cos(x) dx
= sin(\pi/2) - sin(0) - sin(\pi) + sin(\pi/2)
= 2
$$

# Techniques in integration

1. Anti-differentiation
   $$
   \int f(x) dx = F(x) + C
   $$
2. Integration by Substitution
   $$
   \int f(g(x))\frac{dg(x)}{dx} dx = 
   \int f(u) du =
   F(g(x)) + C
   $$
   - Differentials: $du = \frac{du}{dx} dx = g'(x)dx$,
     where $u = g(x)$
3. Integration by Parts
   $$
   \int f(x) \frac{dg(x)}{dx} =
   f(x)g(x) - \int g(x)\frac{df(x)}{dx} dx
   $$
4. Leibniz Integral Rule (next slide)

## Leibniz Integral Rule

$$
\frac{d}{dt} \int^{b(t)}_{a(t)} f(x, t) dx
= \int^{b(t)}_{a(t)} \frac{\partial}{\partial t}
f(x, t) dx + f(b(t), t)\frac{db(t)}{dt} -
f(a(t), t)\frac{da(t)}{dt}
$$

- If $a(t), b(t)$ are constants
  $$
  \frac{d}{dt}\int_a^b f(x, t) dx =
  \int_a^b \frac{\partial}{\partial t} f(x, t) dx
  $$
- Variable limit form
  $$
  \frac{d}{dt}\int_{a(t)}^{b(t)} f(x) dx =
  f(b(t))\frac{db(t)}{dt}-
  f(a(t))\frac{da(t)}{dt}
  $$

## Integrating infinite bounds

To solve 
$$
\int_{0}^{\infty} f(x) dx
$$

1. Express $\infty$ as $s$
   - i.e. $\int_{0}^{s} f(x) dx$
2. Solve the integration in terms of the symbol $s$
   - i.e. $\int_0^s f(x) dx = F(s) - F(0)$
3. Take limit to infinity
   - i.e. $\lim_{s\rightarrow \infty} F(s) - F(0)$

Note:

- $\int_{-\infty}^{\infty} f(x)dx 
  = \int_{-\infty}^{0} f(x) dx + \int_{0}^\infty f(x) dx$
